Clean-up SplitsSound

uniana/cfg/EEdge.v
@@ -4,73 +4,140 @@ Require Import PropExtensionality Lia.
 (** * Kinds of edges in a redCFG **)
 
 Section cfg.
-Context `{C : redCFG}.
+  Context `{C : redCFG}.
 
-Inductive Edge (p q : Lab) : Type :=
-| Enormal : basic_edge p q -> Edge p q
-| Eback : back_edge p q -> Edge p q
-| Eentry : entry_edge p q -> Edge p q
-| Eexit : eexit_edge p q -> Edge p q.
+  Infix "-->" := edge__P.
 
-Lemma Edge_disj (p q : Lab) (H Q : Edge p q)
-  : H = Q.
-Proof.
-  destruct H,Q.
-  all: match goal with
-       | |- ?x _ = ?x _ => f_equal;eapply proof_irrelevance
-       | |- _ => exfalso
-       end.
-  all: unfold back_edge,entry_edge, eexit_edge, exit_edge, basic_edge in *.
-  all: unfold_edge_op' b; unfold_edge_op' b0; repeat destructH;
-    try contradiction.
-  7,10:eapply no_exit_head;unfold exit_edge;eauto.
-  4,8:exfalso;eapply no_exit_head;eexists;eauto; unfold back_edge; unfold_edge_op; eauto.
-  all: lazymatch goal with
-       | H : ~ loop_contains ?q ?p,
-             Q : eq_loop ?p ?q |- _ => eapply H; rewrite Q; eapply loop_contains_self;eauto
-       | H : eq_loop ?p ?q,
-             Q : ~ loop_contains _ ?q |- _ => rewrite <-H in Q; contradiction
-       | _ : loop_head ?q,
-             H : ~ loop_contains ?q ?p,
-                 _ : ~ a_edge__P ?p ?q |- _
-         => eapply H; specialize (back_edge_eq_loop (p:=p) (h:=q)) as Q;
-             exploit Q;[firstorder|rewrite Q;eapply loop_contains_self;eauto]
-       | _ => idtac
-       end.
-Qed.
+  Inductive Edge (p q : Lab) : Type :=
+  | Enormal : basic_edge p q -> Edge p q
+  | Eback : back_edge p q -> Edge p q
+  | Eentry : entry_edge p q -> Edge p q
+  | Eexit : eexit_edge p q -> Edge p q.
 
-Lemma edge_Edge : forall (p q : Lab), edge__P p q -> Edge p q.
-Proof.
-  intros ? ? Hedge.
-  decide (deq_loop p q).
-  - decide (deq_loop q p).
-    + decide (a_edge__P p q).
-      * econstructor;eauto;split;eauto;split;eauto.
-      * eapply Eback. refine (conj Hedge n).
-    + eapply Eexit.
-      simpl_dec' n. simpl_dec' n. destructH.
-      exists x. split;eauto.
-  - eapply Eentry.
-    unfold entry_edge. split_conj;eauto.
-    + simpl_dec' n. simpl_dec' n. destructH.
-      enough (x = q).
-      * subst. eapply loop_contains_loop_head;eauto.
-      * eapply dom_loop_contains in n1 as Hdom;eauto.
-        specialize (PathSingle edge__P p) as Hpath.
-        eapply PathCons in Hedge;eauto.
-        eapply Hdom in Hedge. destruct Hedge;subst;auto.
-        exfalso. cbn in H; destruct H;[|auto]. subst.
-        eapply n1. eapply loop_contains_self;eapply loop_contains_loop_head;eauto.
-    + contradict n. eapply loop_contains_deq_loop;auto.
-Defined.
+  Lemma Edge_disj (p q : Lab) (H Q : Edge p q)
+    : H = Q.
+  Proof.
+    destruct H,Q.
+    all: match goal with
+         | |- ?x _ = ?x _ => f_equal;eapply proof_irrelevance
+         | |- _ => exfalso
+         end.
+    all: unfold back_edge,entry_edge, eexit_edge, exit_edge, basic_edge in *.
+    all: unfold_edge_op' b; unfold_edge_op' b0; repeat destructH;
+      try contradiction.
+    7,10:eapply no_exit_head;unfold exit_edge;eauto.
+    4,8:exfalso;eapply no_exit_head;eexists;eauto; unfold back_edge; unfold_edge_op; eauto.
+    all: lazymatch goal with
+         | H : ~ loop_contains ?q ?p,
+               Q : eq_loop ?p ?q |- _ => eapply H; rewrite Q; eapply loop_contains_self;eauto
+         | H : eq_loop ?p ?q,
+               Q : ~ loop_contains _ ?q |- _ => rewrite <-H in Q; contradiction
+         | _ : loop_head ?q,
+               H : ~ loop_contains ?q ?p,
+                   _ : ~ a_edge__P ?p ?q |- _
+           => eapply H; specialize (back_edge_eq_loop (p:=p) (h:=q)) as Q;
+               exploit Q;[firstorder|rewrite Q;eapply loop_contains_self;eauto]
+         | _ => idtac
+         end.
+  Qed.
 
-Lemma Edge_eq (p q : Lab)
-      (H : edge__P p q)
-      (Q : edge__P p q)
-  : edge_Edge H = edge_Edge Q.
-Proof.
-  erewrite Edge_disj. reflexivity.
-Qed.
+  Lemma edge_Edge : forall (p q : Lab), edge__P p q -> Edge p q.
+  Proof.
+    intros ? ? Hedge.
+    decide (deq_loop p q).
+    - decide (deq_loop q p).
+      + decide (a_edge__P p q).
+        * econstructor;eauto;split;eauto;split;eauto.
+        * eapply Eback. refine (conj Hedge n).
+      + eapply Eexit.
+        simpl_dec' n. simpl_dec' n. destructH.
+        exists x. split;eauto.
+    - eapply Eentry.
+      unfold entry_edge. split_conj;eauto.
+      + simpl_dec' n. simpl_dec' n. destructH.
+        enough (x = q).
+        * subst. eapply loop_contains_loop_head;eauto.
+        * eapply dom_loop_contains in n1 as Hdom;eauto.
+          specialize (PathSingle edge__P p) as Hpath.
+          eapply PathCons in Hedge;eauto.
+          eapply Hdom in Hedge. destruct Hedge;subst;auto.
+          exfalso. cbn in H; destruct H;[|auto]. subst.
+          eapply n1. eapply loop_contains_self;eapply loop_contains_loop_head;eauto.
+      + contradict n. eapply loop_contains_deq_loop;auto.
+  Defined.
+
+  Lemma Edge_eq (p q : Lab)
+        (H : edge__P p q)
+        (Q : edge__P p q)
+    : edge_Edge H = edge_Edge Q.
+  Proof.
+    erewrite Edge_disj. reflexivity.
+  Qed.
+
+
+  Lemma basic_edge_loop_contains a b x
+        (Hedge : basic_edge a b)
+        (Hinner : loop_contains x a)
+    : loop_contains x b.
+  Proof.
+    specialize (loop_contains_loop_head Hinner) as Hhead.
+    destruct Hedge as [Hedge _].
+    eauto using loop_contains_deq_loop, deq_loop_head_loop_contains, eq_loop1.
+  Qed.
+
+  Lemma enter_exit_same e h b c
+        (Hentry : entry_edge e h)
+        (Hexit: exit_edge h b c)
+    : eq_loop c e.
+  Proof.
+    enough (forall h, loop_contains h e <-> loop_contains h c).
+    - unfold eq_loop, deq_loop.
+      firstorder 0.
+    - intros h'. split; intros.
+      + eapply exit_edge_in_loop; try eassumption.
+        * eapply deq_loop_entry in Hentry. unfold deq_loop in Hentry. eauto.
+        * intro. subst. eapply Hentry. assumption.
+      + specialize (deq_loop_exited' Hexit) as Hdeq. unfold deq_loop in Hdeq.
+        edestruct (deq_loop_entry_or Hentry); eauto.
+        subst. unfold exit_edge in Hexit.
+        exfalso. destruct Hexit as [_ [Hexit _]]. contradiction.
+  Qed.
+
+  Lemma not_deq_edge_is_exit a b h
+        (Edge : a --> b)
+        (Hinner : innermost_loop h a)
+        (Hndeq : ~ deq_loop b a)
+    : exit_edge h a b.
+  Proof.
+    eapply edge_Edge in Edge.
+    inv Edge.
+    - exfalso. destruct H as [H _]. eapply Hndeq. eapply eq_loop1. eapply H. reflexivity.
+    - exfalso. eapply back_edge_eq_loop in H. eapply Hndeq. eapply eq_loop1. eapply H. reflexivity.
+    - exfalso. eapply deq_loop_entry in H. contradiction.
+    - destruct H as [h' Hexit].
+      enough (h = h').
+      + subst h'. eassumption.
+      + eauto using exit_edge_innermost, innermost_unique.
+  Qed.
+
+  Lemma ncont_cont_is_entry_edge h a b
+        (Hcont : loop_contains h b)
+        (Hncont : ~ loop_contains h a)
+        (Hedge : a --> b)
+    : entry_edge a b /\ b = h.
+  Proof.
+    eapply edge_Edge in Hedge.
+    inv Hedge.
+    - destruct H as [H _]. rewrite H in Hncont. contradiction.
+    - eapply back_edge_eq_loop in H. rewrite H in Hncont. contradiction.
+    - split; try eassumption. unfold entry_edge in H.
+      destruct H as [_ [Hncontba Hedge]].
+      eauto using entry_through_header.
+    - destruct H as [h' Hexit].
+      eapply deq_loop_exited in Hexit.
+      exfalso. unfold deq_loop in Hexit. eauto.
+  Qed.
+
 End cfg.
 
 Ltac edge_excl
