uniana/cfg/ContractPath.v
@@ -1,0 +1,224 @@
+Require Export HeadRewire PPexhead.
+Require Import Lia.
+
+Section cfg.
+  Context `{C : redCFG}.
+
+  Infix "-->" := edge__P.
+
+
+  Lemma contract_cpath (π : list Lab) p q
+        (Hπ : CPath p q π)
+        (Hdeq : forall x, x ∈ π -> deq_loop x q)
+        (Hnin : forall x, x ∈ tl π -> ~ loop_contains x q) (* Header of q is not on π *)
+    : exists ϕ, HPath p q ϕ /\ ϕ ⊆ π.
+  Proof.
+    revert dependent q. revert dependent π.
+    specialize (well_founded_ind (R:=(@StrictPrefix' Lab)) (@StrictPrefix_well_founded Lab)
+                                 (fun π : list Lab => forall q, CPath p q π ->
+                                                        (forall x, x ∈ π -> deq_loop x q) ->
+                                                        (forall x, x ∈ tl π -> ~ loop_contains x q) ->
+                                                        exists ϕ, HPath p q ϕ /\ ϕ ⊆ π))
+      as WFind.
+    eapply WFind.
+    intros π IH q Hπ Hdeq Hnin. clear WFind.
+    inv Hπ.
+    - exists [q]. unfold incl. split; eauto; econstructor.
+    - specialize (edge_Edge H0) as Hedge.
+      rename H into Hπ. rename q into c. rename π0 into π.
+      assert (Hprefix : StrictPrefix' π (c :: π)) by (repeat econstructor).
+      simpl in Hnin.
+      inv Hedge.
+      + edestruct IH as [ϕ [Hϕ Hincl]]; try eauto.
+        * unfold deq_loop in *. eauto using basic_edge_loop_contains.
+        * intros. intro. eapply Hnin. simpl. eapply in_tl_in. eassumption.
+          eauto using basic_edge_loop_contains.
+        * exists (c :: ϕ). split; [| eauto using incl_app ].
+          econstructor; [ eassumption |].
+          left. split; [ eassumption |].
+          intro.  eapply (Hnin b). eauto using path_contains_front.
+          eauto using loop_contains_self, basic_edge_loop_contains.
+      + edestruct IH as [ϕ [Hϕ Hincl]]; try eauto.
+        * unfold deq_loop in *. eauto using back_edge_loop_contains.
+        * intros. intro. eapply Hnin. simpl. eapply in_tl_in. eassumption.
+          eauto using back_edge_loop_contains.
+        * exists (c :: ϕ). split; [| eauto using incl_app ].
+          econstructor; [ eassumption |].
+          left. split; eauto using back_edge_src_no_loop_head.
+      + unfold entry_edge in H. destruct H as [Hhead [H _]].
+        exfalso. apply H. unfold deq_loop in Hdeq.
+        eauto using loop_contains_self, in_cons, path_contains_front.
+      + destruct H as [h Hexit].
+        decide (h ∈ π) as [ Hhin | Hhnin ].
+        * specialize (in_path_ex_prefix_not_in Hπ Hhin) as Hfirst.
+          destruct Hfirst as [ϕ [Hpre Hninϕ]].
+          destruct ϕ as [ | e ϕ ].
+          -- assert (Heq : p = h) by (eauto using prefix_singleton).
+             subst p. exists [c; h]. split.
+             ++ econstructor; [ econstructor |]. right. exists b. eassumption.
+             ++ unfold incl. intros. inversion H.
+                ** subst. eauto.
+                ** inversion H1. subst. eauto. inversion H2.
+          -- assert (Hedge : e --> h).
+             { eapply prefix_edge_exists. 2:eauto. eauto. }
+             assert (Hedge' : entry_edge e h \/ back_edge e h). {
+               eapply edge_Edge in Hedge.
+               inv Hedge; try eauto.
+               - exfalso. eapply basic_edge_no_loop2. eapply H.
+                 eapply loop_contains_loop_head. eapply Hexit.
+               - destruct H as [h' H]. eapply no_exit_head in H.
+                 exfalso. apply H. unfold loop_contains in Hexit. unfold loop_head. firstorder.
+             }
+             destruct Hedge' as [Hent | Hback].
+             ++ edestruct (@IH (e :: ϕ)) as [ϕ' [Hϕ' Hincl']].
+                ** econstructor. eapply PreStep. eassumption.
+                ** eapply prefix_cons in Hpre. eapply path_prefix_path'; try eassumption.
+                ** intros. eapply eq_loop2.
+                   --- eauto using enter_exit_same.
+                   --- eapply Hdeq. eauto using in_prefix_in.
+                ** simpl. intros. intro. eapply Hnin. eapply in_prefix_in. eapply H.
+                   eauto using prefix_cons. eapply eq_loop2. eauto using enter_exit_same.
+                   eapply deq_loop_refl. eassumption.
+                ** exists (c :: h :: ϕ'). split.
+                   --- econstructor. econstructor. eapply Hϕ'.
+                       +++ left. split; [ eauto |].
+                           intro. eapply (Hnin e).
+                           *** eauto using prefix_cons, in_prefix_in.
+                           *** eauto using deq_loop_head_loop_contains, eq_loop2, enter_exit_same.
+                       +++ right. exists b. eassumption.
+                   --- intros x Hx.
+                       destruct Hx.
+                       +++ subst. left;auto.
+                       +++ destruct H.
+                           *** subst. right;auto.
+                           *** right. eapply prefix_incl;eauto.
+             ++ assert (Hnin2 : forall x, x ∈ (e :: ϕ) -> ~ loop_contains x e). {
+                  intros. intro. eapply Hnin. eapply in_prefix_in.
+                  2: eapply Hpre.
+                  1: eapply in_cons. eassumption.
+                  specialize (back_edge_innermost Hback) as Hinner1.
+                  - enough (x <> h).
+                    + eapply (exit_edge_in_loop Hexit); try eassumption.
+                      eauto using back_edge_loop_contains, eq_loop2.
+                    + intro. subst. contradiction.
+                }
+                edestruct (@IH (e :: ϕ)) as [ϕ' [Hϕ' Hincl']].
+                ** econstructor. eapply PreStep. eassumption.
+                ** eapply prefix_cons in Hpre. eapply path_prefix_path'; try eassumption.
+                ** eauto using exit_edge_innermost, back_edge_innermost,
+                   path_no_loop_head_deq, prefix_cons, path_prefix_path' .
+                ** eauto.
+                ** exists (c :: h :: ϕ'). split.
+                   --- econstructor. econstructor. eapply Hϕ'.
+                       +++ left. split; [ eauto |].
+                           decide (loop_head e); [| eassumption ]. exfalso.
+                           eapply (Hnin2 e); eauto using loop_contains_self.
+                       +++ right. exists b. eassumption.
+                   --- intros x Hx.
+                       destruct Hx.
+                       +++ subst. left;auto.
+                       +++ destruct H.
+                           *** subst. right; auto.
+                           *** right. eapply prefix_incl; eauto.
+        * edestruct (IH π) as [ϕ [Hϕ Hincl]].
+          -- econstructor. econstructor.
+          -- eauto.
+          -- eauto using exit_edge_innermost, back_edge_innermost, path_no_loop_head_deq.
+          -- intros. intro. eapply Hnin. simpl. eapply in_tl_in. eassumption.
+             edestruct (deq_loop_exit_or Hexit); try eassumption.
+             subst. exfalso. eauto using in_tl_in.
+          -- exists (c :: ϕ). split; [| eauto using incl_app ].
+             econstructor; [ eassumption |]. left. split; [ assumption |]. intro.
+             enough (h = b).
+             ++ subst b. eauto using path_contains_front.
+             ++ assert (Heq : eq_loop h b) by (eauto using eq_loop_exiting).
+                assert (Hinner : innermost_loop h b) by (eauto using exit_edge_innermost).
+                eapply loop_contains_self in H.
+                destruct Hinner as [Hinner _].
+                eauto using head_unique.
+  Qed.
+
+  Lemma contract_cpath' (π : list Lab) q p
+        (Hπ : CPath p q π)
+        (Hdeq : deq_loop p q)
+        (Hnin : forall x, x ∈ tl π -> ~ loop_contains x q)
+    : exists ϕ, HPath p q ϕ /\ ϕ ⊆ π.
+  Proof.
+    eapply contract_cpath;eauto.
+    unfold deq_loop. intros x Hxin h Hhcont.
+    decide (loop_contains h x) as [Htmp | Hxcont]; [ assumption |].
+    exfalso.
+    destruct π as [|l π']; [ contradiction |].
+    replace l with q in * by (eauto using path_front).
+    simpl in Hnin.
+    inversion Hπ; subst. {
+      inv Hxin. contradiction. inv H.
+    }
+    rename H3 into Hedge. rename H0 into Hπ'.
+    destruct Hxin as [Htmp | Hxin]. {
+      subst. contradiction.
+    }
+    decide (loop_contains q q) as [Hhead | Hnhead ].
+    - (* if q is a loop header, we cannot use Hnin to create a contradiction because it
+         is only applicable to tl π. We essentially need to show that there is a header
+         that contains q and lies on π' that contains all nodes on π'.
+         We get that header using p_p_ex_head. Then, the fact that this header
+         contains all other loops is in contradiction with Hnin. *)
+      edestruct loop_reachs_member as [ρ Hρ].
+      eapply (deq_loop_head_loop_contains Hdeq).
+      eauto using loop_contains_loop_head.
+      remember ((q :: π') ++ tl ρ) as σ.
+      assert (Hσ : CPath q q σ). {
+        rewrite Heqσ.
+        eapply path_app'.
+        - eapply subgraph_path'; eauto using a_edge_incl.
+        - eassumption.
+      }
+      edestruct (p_p_ex_head Hσ) as [ho [Hin Hcont]]. {
+        rewrite Heqσ. simpl.
+        induction π'; try contradiction.
+        simpl. lia.
+      }
+      assert (Hne : q <> ho). {
+        intro. subst ho.
+        eapply Hxcont.
+        eapply loop_contains_trans.
+        eapply Hhcont. eapply Hcont.
+        rewrite Heqσ.
+        eauto using in_or_app.
+      }
+      assert (Hoinπ' : ho ∈ π'). {
+        (* Show that ho is on the π' part of σ.
+           Essentially by constructing an acyclic path from ho to ho. *)
+        assert (Hinσ := Hin).
+        rewrite Heqσ in Hin. simpl in Hin.
+        destruct Hin.
+        - exfalso. eauto.
+        - eapply in_app_or in H.
+          destruct H;[ eassumption |].
+          exfalso.
+          edestruct loop_reachs_member as [τ Hτ]. {
+            eapply Hcont. rewrite Heqσ. simpl. left. reflexivity.
+          }
+          eapply in_tl_in in H.
+          edestruct (path_to_elem Hρ H) as [ω [Hω _]].
+          eapply (path_path_acyclic Hτ Hω); eauto.
+      }
+      eapply (Hnin _ Hoinπ').
+      eapply Hcont.
+      rewrite Heqσ. eauto.
+    - (* the other case is simple. The path needs to go through the loop header h
+         to reach p. This header contradicts Hnin. *)
+      eapply path_from_elem in Hπ'; try eauto.
+      destruct Hπ' as [ϕ [Hϕ Hpost]].
+      eapply (Hnin h); try eassumption.
+      eapply in_postfix_in; try eassumption.
+      eapply (dom_loop_contains).
+      2: eapply Hxcont.
+      2: eapply Hϕ.
+      eapply (preds_in_same_loop Hhcont). {
+        intro. subst. eauto.
+      }
+      eassumption.
+  Qed.
+End cfg.
