uniana/cfg/PPexhead.v
@@ -1,0 +1,35 @@
+Require Export CFGinnermost.
+
+Section cfg.
+  Context `(C : redCFG).
+  (** ** p p ex head **)
+
+  Lemma p_p_ex_head' (p q : Lab) π ϕ
+        (Hpath : CPath p q π)
+        (Hdeq : forall x, x ∈ π -> deq_loop p x)
+        (Hacy : APath q p ϕ)
+        (Hlen : | π | >= 2)
+  : exists h, h ∈ π /\ forall x, x ∈ π -> loop_contains h x.
+  Proof.
+  (* by induction on π:
+   * * if nil,singleton: contradiction
+   * * if doubleton: easy style: h=q, bc of APath p-->q must be a back_edge, thus loop_contains q p
+   * * else:
+   * * edge distinction for ? --> q:
+   *   * if back_edge then: we have found h
+   *   * otw. IH
+   *)
+  Admitted.
+
+  Lemma p_p_ex_head (p : Lab) π
+        (Hpath : CPath p p π)
+        (Hlen : | π | >= 2)
+    : exists h, h ∈ π /\ forall x, x ∈ π -> loop_contains h x.
+  Proof.
+    (* implode π wrt. p then Hdeq of p_p_ex_head' holds and the conclusion is extendable from there *)
+    eapply p_p_ex_head';eauto.
+    - admit.
+    - econstructor.
+  Admitted.
+
+End cfg.
